lib/extra/Array.v
@@ -17,6 +17,7 @@ Parameter length : forall T, array T -> nat.
 Parameter read : forall T `{Inhab T}, array T -> nat -> T.
 Parameter write : forall T, array T -> nat -> T -> array T.
 
+Parameter empty : forall T, array T.
 Parameter from_list : forall T, list T -> array T.
 Parameter to_list : forall T, array T -> list T.
 
@@ -31,6 +32,9 @@ Parameter read_write_neq : forall T `{Inhab T} a (t : T) n1 n2,
 
 Parameter write_length : forall T a (t : T) n,
   length (write a n t) = length a.
+
+Parameter empty_length : forall T,
+  length (empty T) = 0.
 
 Parameter from_list_length : forall T (l : list T),
   length (from_list l) = LibList.length l.
@@ -77,6 +81,9 @@ Definition write T (a : array T) n t := update n t a : array T.
 Definition from_list T := id : list T -> array T.
 Definition to_list T := id : array T -> list T.
 
+Definition empty T := from_list nil : array T.
+Arguments empty [T].
+
 Lemma read_write_eq : forall T `{Inhab T} a (t : T) n,
   n < length a ->
   read (write a n t) n = t.
@@ -98,6 +105,10 @@ Proof. reflexivity. Qed.
 
 Lemma to_list_length : forall T (a : array T),
   LibList.length (to_list a) = length a.
+Proof. reflexivity. Qed.
+
+Lemma empty_length : forall T,
+  length (@empty T) = 0.
 Proof. reflexivity. Qed.
 
 Lemma from_list_read : forall T `{Inhab T} (l : list T) n,
