low/InternalTypes.v
@@ -1,0 +1,126 @@
+(** InternalTypes.
+  This file describes various internal data types used in the source of R. **)
+
+Require Import Rinternals Monads.
+
+
+(** * FUNTAB **)
+
+(** This section defines the FUNTAB structure, which is used to store
+  primitive and internal functions, as well as some constructs to
+  evaluate it. Most of these constructs can be found in
+  include/Defn.h. **)
+
+(** All function in the array [R_FunTab] have the same type. **)
+Definition function_code :=
+  state ->
+  SExpRec_pointer -> (** call **)
+  SExpRec_pointer -> (** op **)
+  SExpRec_pointer -> (** args **)
+  SExpRec_pointer -> (** rho **)
+  result SExpRec_pointer.
+
+(** The following type is represented in C as an integer, each of its figure
+  (in base 10) representing a different bit of information. **)
+Record funtab_eval_arg := make_funtab_eval_arg {
+    funtab_eval_arg_internal : bool ; (** Whether it is stored in the array [.Internals] or directly visible. **)
+    funtab_eval_arg_eval : bool (** Whether its arguments should be evaluated before calling. **)
+  }.
+
+(** PPkind **)
+Inductive PPkind :=
+  | PP_INVALID
+  | PP_ASSIGN
+  | PP_ASSIGN2
+  | PP_BINARY
+  | PP_BINARY2
+  | PP_BREAK
+  | PP_CURLY
+  | PP_FOR
+  | PP_FUNCALL
+  | PP_FUNCTION
+  | PP_IF
+  | PP_NEXT
+  | PP_PAREN
+  | PP_RETURN
+  | PP_SUBASS
+  | PP_SUBSET
+  | PP_WHILE
+  | PP_UNARY
+  | PP_DOLLAR
+  | PP_FOREIGN
+  | PP_REPEAT
+  .
+
+Instance PPkind_Comparable : Comparable PPkind.
+  prove_comparable_trivial_inductive.
+Defined.
+
+Instance PPkind_Inhab : Inhab PPkind.
+  apply prove_Inhab. constructors~.
+Qed.
+
+(** PPprec **)
+Inductive PPprec :=
+  | PREC_FN
+  | PREC_EQ
+  | PREC_LEFT
+  | PREC_RIGHT
+  | PREC_TILDE
+  | PREC_OR
+  | PREC_AND
+  | PREC_NOT
+  | PREC_COMPARE
+  | PREC_SUM
+  | PREC_PROD
+  | PREC_PERCENT
+  | PREC_COLON
+  | PREC_SIGN
+  | PREC_POWER
+  | PREC_SUBSET
+  | PREC_DOLLAR
+  | PREC_NS
+  .
+
+Instance PPprec_Comparable : Comparable PPprec.
+  prove_comparable_trivial_inductive.
+Defined.
+
+Instance PPprecd_Inhab : Inhab PPprec.
+  apply prove_Inhab. constructors~.
+Qed.
+
+(** PPinfo **)
+Record PPinfo := make_PPinfo {
+    PPinfo_kind : PPkind ;
+    PPinfo_precedence : PPprec ;
+    PPinfo_rightassoc : bool
+  }.
+
+(** FUNTAB **)
+Record funtab_cell := make_funtab_cell {
+    fun_name : string ;
+    fun_cfun : function_code ;
+    fun_code : int ; (** The number stored here can be quite large. We thus use [int] instead of [nat] here. **)
+    fun_eval : funtab_eval_arg ;
+    fun_arity : int ;
+    fun_gram : PPinfo
+  }.
+
+Definition funtab := option (list funtab_cell).
+
+
+(** * Type2Table **)
+
+(** These definitions can be found in the file main/util.c. **)
+
+Record Type2Table_type := make_Type2Table_type {
+    Type2Table_cstrName : string ;
+    Type2Table_rcharName : SExpRec_pointer ;
+    Type2Table_rstrName : SExpRec_pointer ;
+    Type2Table_rsymName : SExpRec_pointer ;
+  }.
+
+Instance Type2Table_type_Inhab : Inhab Type2Table_type.
+  apply prove_Inhab. constructors; apply arbitrary.
+Qed.
