low/Rparsing.v
@@ -20,7 +20,7 @@ Section Parameters.
 
 Variable globals : Globals.
 
-Let read_globals : GlobalVariable -> SExpRec_pointer := globals.
+Let read_globals := read_globals globals.
 
 Local Coercion read_globals : GlobalVariable >-> SExpRec_pointer.
 
